src/ASN1.Low.Value.OID.fst
@@ -112,7 +112,7 @@ let seq_of_oid_buffer
 = lemma_known_oids_as_seq_contains_oid_seq_of oid;
   oid_seq_of oid
 
-// #push-options "--query_stats --z3rlimit 32"
+// #push-options "--z3rlimit 32"
 // inline_for_extraction
 // let blit_from_ib
 //   (len: size_t)
@@ -185,7 +185,7 @@ let seq_of_oid_buffer
 
 
 #restart-solver
-#push-options "--query_stats --z3rlimit 64 --fuel 2 --ifuel 1"
+#push-options "--z3rlimit 64 --fuel 2 --ifuel 1"
 inline_for_extraction
 let serialize32_asn1_oid_backwards
   (len: asn1_value_int32_of_type OID)
