src/RIoT.Base.fst
@@ -1,0 +1,97 @@
+module RIoT.Base
+
+open LowStar.Comment
+
+module Fail = LowStar.Failure
+module B = LowStar.Buffer
+module IB = LowStar.ImmutableBuffer
+module HS  = FStar.HyperStack
+module HST = FStar.HyperStack.ST
+
+module SHA2 = Hacl.Hash.SHA2
+module HMAC = Hacl.HMAC
+module HKDF = Hacl.HKDF
+module ECDSA = Hacl.Impl.ECDSA
+// module P256 = Hacl.Impl.P256
+module Ed25519 = Hacl.Ed25519
+module Curve25519 = Hacl.Curve25519_51
+
+// module HW = HWAbstraction
+open RIoT.Declassify
+open Lib.IntTypes
+open Spec.Hash.Definitions
+open Hacl.Hash.Definitions
+(*
+ * Some common definitions used in the RIoT code
+ *)
+
+#set-options "--__temp_no_proj RIoT.Definitions"
+
+(* ZT: restrict it to `SHA2_256` for convenience,
+       because `Hacl.Curve25519` only support it *)
+type riot_hash_alg = a:hash_alg{a == SHA2_256}
+
+inline_for_extraction
+let alg : riot_hash_alg = SHA2_256
+
+inline_for_extraction noextract
+let riot_hash (alg:riot_hash_alg) : hash_st alg =
+  match alg with
+  | SHA2_256 -> Hacl.Hash.SHA2.hash_256
+  | SHA2_384 -> Hacl.Hash.SHA2.hash_384
+  | SHA2_512 -> Hacl.Hash.SHA2.hash_512
+  | SHA1     -> Hacl.Hash.SHA1.legacy_hash
+
+inline_for_extraction noextract
+let riot_hmac (alg:riot_hash_alg) : Hacl.HMAC.compute_st alg =
+  match alg with
+  | SHA2_256 -> Hacl.HMAC.compute_sha2_256
+  | SHA2_384 -> Hacl.HMAC.compute_sha2_384
+  | SHA2_512 -> Hacl.HMAC.compute_sha2_512
+  | SHA1     -> Hacl.HMAC.legacy_compute_sha1
+
+unfold let digest_len = hash_len alg
+
+unfold type digest_t = hash_t alg
+
+unfold type hashable_len = i:size_t{0 < v i /\ v i <= max_input_length alg}
+
+unfold let cdi_len = digest_len
+
+unfold let byte_sec = uint8
+unfold let byte_pub = pub_uint8
+
+unfold let bytes_pub  = Seq.seq byte_pub
+unfold let lbytes_pub = Seq.lseq byte_pub
+unfold let bytes_sec  = Seq.seq byte_sec
+unfold let lbytes_sec = Seq.lseq byte_sec
+
+// #push-options "--z3rlimit 32"
+// let label_DeviceID_l: list byte_sec = [u8 0; u8 0]
+// let label_DeviceID_len
+// : len: size_t { valid_hkdf_lbl_len len /\
+//                 v len == List.length label_DeviceID_l }
+// = assert_norm (valid_hkdf_lbl_len 2ul);
+//   assert_norm (List.length label_DeviceID_l == 2);
+//   2ul
+// let label_DeviceID
+// : ib:IB.libuffer uint8 (v label_DeviceID_len) (Seq.createL label_DeviceID_l)
+//   { IB.frameOf ib == HS.root /\ IB.recallable ib /\
+//     valid_hkdf_lbl_len (B.len ib) }
+// = assert_norm (valid_hkdf_lbl_len label_DeviceID_len);
+//   IB.igcmalloc_of_list HS.root label_DeviceID_l
+
+// let label_AliasKey_l: list byte_sec = [u8 1; u8 1]
+// let label_AliasKey_len
+// : len: size_t { valid_hkdf_lbl_len len /\
+//                 v len == List.length label_AliasKey_l }
+// = assert_norm (valid_hkdf_lbl_len 2ul);
+//   assert_norm (List.length label_AliasKey_l == 2);
+//   2ul
+// let label_AliasKey
+// : ib:IB.libuffer uint8 (v label_AliasKey_len) (Seq.createL label_AliasKey_l)
+//   { IB.frameOf ib == HS.root /\ IB.recallable ib /\
+//     valid_hkdf_lbl_len (B.len ib) }
+// = assert_norm (valid_hkdf_lbl_len label_AliasKey_len);
+//   IB.igcmalloc_of_list HS.root label_AliasKey_l
+// #push-options
