src/RIoT.Impl.Crypto.fst
@@ -1,0 +1,167 @@
+module RIoT.Impl.Crypto
+
+module Fail = LowStar.Failure
+module B = LowStar.Buffer
+module IB = LowStar.ImmutableBuffer
+module HS  = FStar.HyperStack
+module HST = FStar.HyperStack.ST
+
+module SHA2 = Hacl.Hash.SHA2
+module HMAC = Hacl.HMAC
+module HKDF = Hacl.HKDF
+module Ed25519 = Hacl.Ed25519
+open Spec.Hash.Definitions
+open Hacl.Hash.Definitions
+open Lib.IntTypes
+
+open RIoT.Base
+open RIoT.Declassify
+open RIoT.Spec.Crypto
+
+#set-options "--z3rlimit 64 --fuel 0 --ifuel 0"
+
+let derive_key_pair
+  (public_key : B.lbuffer pub_uint8 32)                 // Out
+  (private_key: B.lbuffer uint8 32)                     // Out
+                    (* NOTE Not using lbuffer here because lbuffer doesn't accept null *)
+  (ikm_len: size_t) (ikm: B.buffer uint8 {B.length ikm == v ikm_len})  // In: Initial Data for derivation
+  (lbl_len: size_t) (lbl: B.buffer uint8 {B.length lbl == v lbl_len})  // In: Label for derivation
+: HST.Stack unit
+  (requires fun h -> let alg = SHA2_256 in
+    (* Separation Logic Properties *)
+    B.live h ikm /\ B.live h lbl /\ B.live h public_key /\ B.live h private_key /\
+    B.all_disjoint [B.loc_buffer ikm;
+                    B.loc_buffer lbl;
+                    B.loc_buffer public_key;
+                    B.loc_buffer private_key] /\
+
+    (* for Hacl.HKDF.extract_st *)
+    v ikm_len + block_length alg < pow2 32 /\
+    (* for Spec.Agile.HKDF.extract *)
+    v ikm_len + block_length alg <= max_input_length alg /\
+    (* for Hacl.HKDF.expand_st *)
+    hash_length alg + v lbl_len + 1 + block_length alg < pow2 32 /\
+    (* for Spec.Aigle.HKDF.expand *)
+    hash_length alg + v lbl_len + 1 + block_length alg < max_input_length alg)
+  (ensures  fun h0 _ h1 -> let alg = SHA2_256 in
+    B.(modifies ((loc_buffer public_key) `loc_union` (loc_buffer private_key)) h0 h1) /\
+   (let pub_seq, priv_seq = derive_key_pair_spec ikm_len (B.as_seq h0 ikm) lbl_len (B.as_seq h0 lbl) in
+    B.as_seq h1 public_key == pub_seq /\ B.as_seq h1 private_key == priv_seq ))
+= HST.push_frame ();
+
+  (* NOTE:  Using SHA2_256 because Curve25519/Ed25519 requires a 32-bit private key *)
+  let alg = SHA2_256 in
+
+  (* Using an empty (0x00) buffer of hashLen as salt. *)
+  let salt: b:B.lbuffer uint8 32 {Spec.Agile.HMAC.keysized alg (B.length b)} = B.alloca (u8 0x00) (hash_len alg) in
+
+  (* Derive private key from `ikm` and `lbl` using HKDF *)
+  (* Step 1. extract a `prk` (Pseudo Random Key) from an empty `salt` of `hashLen` and `ikm` *)
+  let prk : b:B.lbuffer uint8 32 {B.length b == hash_length alg} = B.alloca (u8 0x00) (hash_len alg) in
+  HKDF.extract_sha2_256
+    prk                 // out: Pseudo Random Key
+    salt (hash_len alg) // in : (optional) Salt
+    ikm  ikm_len;       // in : Input Keying Material
+
+  (* Step 2. expand `prk` and `lbl` to a `okm` (Output Keying Material) *)
+  (**)assert_norm (Spec.Agile.HMAC.keysized alg (hash_length alg));
+  HKDF.expand_sha2_256
+    private_key        // out: Output Keying Material
+    prk (hash_len alg) // in : Pseudo Random Key
+    lbl lbl_len        // in : (optional) Info
+    (hash_len alg);    // in : okm len
+
+  (* Derive public key from private key using Ed25519 (FIXME: Or Curve25519?) *)
+  let secret_public_key: B.lbuffer uint8 32 = B.alloca (u8 0) 32ul in
+  Ed25519.secret_to_public
+    secret_public_key   // out: public
+    private_key; // in : secret
+
+  declassify_secret_buffer
+    (* len *) 32ul
+    (* src *) secret_public_key
+    (* dst *) public_key;
+  HST.pop_frame ()
+
+
+
+let derive_DeviceID
+  (deviceID_pub: B.lbuffer pub_uint8 32)
+  (deviceID_priv: B.lbuffer uint8 32)
+  // (cdi_len: hashable_len)
+  (cdi: B.lbuffer uint8 32)
+  (riot_label_DeviceID_len: size_t {valid_hkdf_lbl_len riot_label_DeviceID_len})
+  (riot_label_DeviceID: B.lbuffer uint8 (v riot_label_DeviceID_len))
+: HST.Stack (unit)
+  (requires fun h ->
+    B.(all_live h [buf deviceID_pub;
+                   buf deviceID_priv;
+                   buf cdi;
+                   buf riot_label_DeviceID]) /\
+    B.(all_disjoint [loc_buffer deviceID_pub;
+                     loc_buffer deviceID_priv;
+                     loc_buffer cdi;
+                     loc_buffer riot_label_DeviceID]))
+  (ensures fun h0 _ h1 ->
+    B.(modifies (loc_buffer deviceID_pub `loc_union` loc_buffer deviceID_priv) h0 h1) /\
+    ((B.as_seq h1 deviceID_pub <: lbytes_pub 32), (B.as_seq h1 deviceID_priv <: lbytes_sec 32)) ==
+    derive_DeviceID_spec (B.as_seq h1 cdi) riot_label_DeviceID_len (B.as_seq h1 riot_label_DeviceID)
+   )
+= HST.push_frame ();
+  let cDigest = B.alloca (u8 0) 32ul in
+  riot_hash alg
+    cdi 32ul
+    cDigest;
+  derive_key_pair
+    deviceID_pub
+    deviceID_priv
+    32ul cDigest
+    riot_label_DeviceID_len riot_label_DeviceID;
+  HST.pop_frame ()
+
+let derive_AliasKey
+  (aliasKey_pub: B.lbuffer pub_uint8 32)
+  (aliasKey_priv: B.lbuffer uint8 32)
+  // (cdi_len: hashable_len)
+  (cdi: B.lbuffer uint8 32)
+  (fwid: B.lbuffer uint8 32)
+  (riot_label_AliasKey_len: size_t {valid_hkdf_lbl_len riot_label_AliasKey_len})
+  (riot_label_AliasKey: B.lbuffer uint8 (v riot_label_AliasKey_len))
+: HST.Stack (unit)
+  (requires fun h ->
+    B.(all_live h [buf aliasKey_pub;
+                   buf aliasKey_priv;
+                   buf cdi;
+                   buf fwid;
+                   buf riot_label_AliasKey]) /\
+    B.(all_disjoint [loc_buffer aliasKey_pub;
+                     loc_buffer aliasKey_priv;
+                     loc_buffer cdi;
+                     loc_buffer fwid;
+                     loc_buffer riot_label_AliasKey]))
+  (ensures fun h0 _ h1 ->
+    B.(modifies (loc_buffer aliasKey_pub `loc_union` loc_buffer aliasKey_priv) h0 h1) /\
+    ((B.as_seq h1 aliasKey_pub  <: lbytes_pub 32),
+     (B.as_seq h1 aliasKey_priv <: lbytes_sec 32)) == derive_AliasKey_spec
+                                                        (B.as_seq h1 cdi)
+                                                        (B.as_seq h1 fwid)
+                                                        riot_label_AliasKey_len
+                                                        (B.as_seq h1 riot_label_AliasKey) /\
+    True
+    )
+= HST.push_frame ();
+  let cDigest = B.alloca (u8 0) 32ul in
+  riot_hash alg
+    cdi 32ul
+    cDigest;
+  let aDigest = B.alloca (u8 0) 32ul in
+  riot_hmac alg
+    aDigest
+    cDigest 32ul
+    fwid    32ul;
+  derive_key_pair
+    aliasKey_pub
+    aliasKey_priv
+    32ul aDigest
+    riot_label_AliasKey_len riot_label_AliasKey;
+  HST.pop_frame ()
