src/RIoT.Spec.Certificate.fst
@@ -1,0 +1,135 @@
+module RIoT.Spec.Certificate
+
+open ASN1.Spec
+open X509
+
+open RIoT.Base
+open RIoT.Declassify
+open RIoT.X509
+
+open Lib.IntTypes
+
+module B32 = FStar.Bytes
+module B = LowStar.Buffer
+module IB = LowStar.ImmutableBuffer
+module HS  = FStar.HyperStack
+module HST = FStar.HyperStack.ST
+
+#set-options "--z3rlimit 32 --fuel 0 --ifuel 0"
+
+(* Create AliasKey To-Be-Signed Certificate
+  =======================================
+  RFC 5280:
+     TBSCertificate  ::=  SEQUENCE  {
+        version         [0]  EXPLICIT Version DEFAULT v1,
+        serialNumber         CertificateSerialNumber,
+        signature            AlgorithmIdentifier,
+        issuer               Name,
+        validity             Validity,
+        subject              Name,
+        subjectPublicKeyInfo SubjectPublicKeyInfo,
+        issuerUniqueID  [1]  IMPLICIT UniqueIdentifier OPTIONAL,
+                             -- If present, version MUST be v2 or v3
+        subjectUniqueID [2]  IMPLICIT UniqueIdentifier OPTIONAL,
+                             -- If present, version MUST be v2 or v3
+        extensions      [3]  EXPLICIT Extensions OPTIONAL
+                             -- If present, version MUST be v3
+        }
+
+   In our case:
+      TBSCertificate  ::=  SEQUENCE  {
+        ----------------
+        |              |
+        |   Template   |
+        |              |
+        ----------------
+        subjectPublicKeyInfo for AliasKey,
+        extensions           for RIoT
+        }
+   NOTE: The SEQUENCE Tag and Length of TBS is __NOT__ part of the template
+   NOTE: Other extensions like Key Usage are __NOT__ included in this version.
+*)
+
+(* A predicate says that the length of created TBS (computed
+   from `template_len` and `version`) is valid, i.e., less than
+   or equal to 2^32 - 6 *)
+unfold
+let valid_aliasKeyTBS_ingredients
+  (template_len: asn1_int32)
+  (version: datatype_of_asn1_type INTEGER)
+= v template_len + length_of_asn1_primitive_TLV version + 155
+  <= asn1_value_length_max_of_type SEQUENCE
+
+let create_aliasKeyTBS_spec
+  (template_len: asn1_int32)
+  (aliasKeyTBS_template: lbytes_pub (v template_len))
+  (version: datatype_of_asn1_type INTEGER
+            { valid_aliasKeyTBS_ingredients template_len version })
+  (fwid: lbytes_sec 32)
+  (deviceID_pub: lbytes_pub 32)
+  (aliasKey_pub: lbytes_pub 32)
+: GTot (aliasKeyTBS_t_inbound template_len)
+=
+(* Create AliasKeyTBS *)
+  let aliasKeyTBS_template32: B32.lbytes32 template_len = B32.hide aliasKeyTBS_template in
+  let deviceID_pub32: B32.lbytes32 32ul = B32.hide deviceID_pub in
+  let fwid32        : B32.lbytes32 32ul = B32.hide (declassify_secret_bytes fwid) in
+  let aliasKey_pub32: B32.lbytes32 32ul = B32.hide aliasKey_pub in
+  let aliasKeyTBS: aliasKeyTBS_t_inbound template_len = x509_get_AliasKeyTBS
+                                                        template_len
+                                                        aliasKeyTBS_template32
+                                                        version
+                                                        fwid32
+                                                        deviceID_pub32
+                                                        aliasKey_pub32 in
+  (* Prf *) lemma_serialize_aliasKeyTBS_size template_len aliasKeyTBS;
+  (* Prf *) lemma_serialize_aliasKeyTBS_sequence_TLV_size_exact template_len aliasKeyTBS;
+
+(* return *) aliasKeyTBS
+
+
+(* Sign and Finalize AliasKey Certificate
+  =======================================
+  RFC 5280:
+   Certificate  ::=  SEQUENCE  {
+        tbsCertificate       TBSCertificate,
+        signatureAlgorithm   AlgorithmIdentifier,
+        signatureValue       BIT STRING  }
+*)
+
+(* A predicate says that
+   1) the length of TBS is valid as Hacl's HKDF message length
+   2) the length of created CRT is valid as our ASN.1 TLV SEQUENCE value length
+*)
+unfold
+let valid_aliasKeyCRT_ingredients
+  (tbs_len: asn1_int32)
+= // (* implied *) v tbs_len + 64 <= max_size_t /\
+  v tbs_len + 76 <= asn1_value_length_max_of_type SEQUENCE
+
+let sign_and_finalize_aliasKeyCRT_spec
+  (deviceID_priv: lbytes_sec 32)
+  (aliasKeyTBS_len: size_t
+                    { valid_aliasKeyCRT_ingredients aliasKeyTBS_len })
+  (aliasKeyTBS_seq: lbytes_pub (v aliasKeyTBS_len))
+: GTot (aliasKeyCRT_t_inbound aliasKeyTBS_len)
+=
+
+(* Classify AliasKeyTBS *)
+  let aliasKeyTBS_seq_sec: lbytes_sec (v aliasKeyTBS_len) = classify_public_bytes aliasKeyTBS_seq in
+
+(* Sign AliasKeyTBS *)
+  let aliasKeyTBS_sig_sec: lbytes_sec 64 = Spec.Ed25519.sign deviceID_priv aliasKeyTBS_seq_sec in
+
+(* Declassify AliasKeyTBS *)
+  let aliasKeyTBS_sig    : lbytes_pub 64 = declassify_secret_bytes aliasKeyTBS_sig_sec in
+
+(* Create AliasKeyCRT with AliasKeyTBS and Signature *)
+  let aliasKeyTBS_seq32  : B32.lbytes32 aliasKeyTBS_len = B32.hide aliasKeyTBS_seq in
+  let aliasKeyTBS_sig32  : x509_signature_raw_t alg_AliasKey = B32.hide aliasKeyTBS_sig in
+  let aliasKeyCRT: aliasKeyCRT_t_inbound aliasKeyTBS_len = x509_get_AliasKeyCRT
+                                                             aliasKeyTBS_len
+                                                             aliasKeyTBS_seq32
+                                                             aliasKeyTBS_sig32 in
+
+(* return *) aliasKeyCRT
